Interior Point Method

#+include: ~/org/latex.org


* Basic Idea

	The idea behind IPM is to relax the complementarity constraint
	arising from the KKT conditions:

	\begin{align}
	 Q x + c& = A^T \lambda \\
	\st \quad 0 \leq A x - b &\bot \   \lambda \geq 0 \\
	\end{align}

	Letting $w = Ax - b$, we require instead that:
	
	\[ W \lambda = \mu \]

	where capitalized variables denote equivalent diagonal matrices. We
	solve the relaxed, non-linear system using Newton's method, then
	decrease $\mu$, and so on until convergence. In practice, we only
	perform one newton step at each iteration.

	In theory we should remain feasible at all times
	

* Equations lol

** Non-linear system
	 
	 \begin{array}{}
	 Qx  &- A^T \lambda &= -c  \\ 
	 Ax  &- \mu \inv{\lambda} &= b\\
	 \end{array}
	 
** Newton

	 \begin{array}{}
	 Qx  &- A^T \lambda \block{\lambda + \dd \lambda} &= -c  \\ 
	 Ax  &+ \mu \lambda^{-2}\dd \lambda &= b + \mu \inv{\lambda} \\
	 \end{array}

	 That is:
	 
	 \begin{array}{}
	 Qx  &- A^T \lambda^\star &= -c  \\ 
	 Ax  &+ \mu \lambda^{-2} \lambda^\star &= b + 2 \mu \inv{\lambda} \\
	 \end{array}


	 This can be rearranged using the Schur complement:

	 \[ \lambda^\star = \frac{\lambda^2}{\mu}\block{ b + 2 \mu \inv{\lambda} - Ax} \]

	 Letting $\eta = \frac{\lambda^2}{\mu}$, this gives:

	 \begin{align}
	 \block{Q + A^T \eta A}x &= -c + A^T \eta \block{b + 2 \mu \inv{\lambda} } \\
	 &=   -c + A^T \block{ \eta b + 2 \lambda }\\
	 \end{align}

	 
	 

* Equations (again)

** System

	\[ \mat{Qx & -A^T \lambda& \\ Ax & & -\omega \\ & \lambda \omega & } = \mat{-c \\ b \\ \mu} \]
	
** Newton

	\[ 
	\mat{Qx & -A^T \lambda& \\ Ax & & -\omega \\ & \bar{\omega}\lambda & + \bar{\lambda}\omega } =
	\mat{-c \\ b \\ \mu + \bar{\lambda \omega}} 
	\]
	 
	\[ 
	\mat{Qx & -A^T \lambda& \\ -\bar{\lambda}Ax & & +\bar{\lambda}\omega \\ & \bar{\omega}\lambda & + \bar{\lambda}\omega } = 
	\mat{-c \\ -\bar{\lambda}b \\ \mu + \bar{\lambda \omega}} 
	\]


	
** Symmetric $m + n$
	
	\[ 
	\mat{Qx & -A^T \lambda& \\ -\bar{\lambda}Ax & -\bar{\omega}\lambda } = 
	\mat{-c \\ -\bar{\lambda}b - \mu - \bar{\lambda \omega}} 
	\]


	\[ 
	\mat{Qx & -A^T \bar{\lambda} \dd \lambda& \\ -\bar{\lambda}Ax & -\bar{\omega \lambda} \dd \lambda } = 
	\mat{-c \\ -\bar{\lambda}b - \mu - \bar{\lambda \omega}} 
	\]

** Symmetric $m$

	 \[ -\lambda = \frac{1}{\bar{\omega} } \block{ \bar{\lambda}\block{A x - b} - \mu } - \bar{\lambda} \]

	 Let $\eta = \frac{ \bar{\lambda} } {\bar{\omega} }$

	 \[ \block{Q + A^T \eta A} x = -c + A^T \block{ \eta b + \bar{\lambda} + \frac{\mu}{\bar{\omega} } } \]
	 
